Restructure FSAT, add some missing proofs

theories/FOL/Semantics/FiniteTarski/Fragment.v
@@ -1,19 +1,16 @@
 From Undecidability.FOL.Semantics Require Import Tarski.FragmentFacts.
+From Undecidability.FOL.Semantics Require Export FiniteTarski.Listability.
 From Undecidability.FOL.Syntax Require Import Facts.
 Require Import Undecidability.Synthetic.DecidabilityFacts.
+Require Import Undecidability.Shared.Dec.
 Require Import List.
 
-#[global]
-Existing Instance falsity_on.
-
 (* Definition of finiteness *)
-
-Definition listable X :=
-  exists L, forall x : X, In x L.
 
 Section DefaultSyntax. (* An alternative development of FSAT in Trakhtenbrot is "Trakhtenbrot Syntax" *)
   Context {Σ_funcs : funcs_signature}.
   Context {Σ_preds : preds_signature}.
+  Context {ff : falsity_flag}.
 
   (* Satisfiability in a finite and decidable model *)
 
@@ -38,3 +35,24 @@ Section DefaultSyntax. (* An alternative development of FSAT in Trakhtenbrot is 
   Definition FSATdc (phi : cform) :=
     FSATd (proj1_sig phi).
 End DefaultSyntax.
+
+Section decidable.
+  Context {Σ_funcs : funcs_signature}.
+  Context {Σ_preds : preds_signature}.
+  Context {ff : falsity_flag}.
+
+  (* Show satisfaction decidable for fixed model *)
+  Lemma general_decider D (I:interp D) (e : env D) f : cListable D -> (forall (ff:falsity_flag) p v ee, dec (ee ⊨ atom p v)) -> dec (e ⊨ f).
+  Proof.
+  intros Hfin Hdec.
+  induction f as [|f p v|f [] l IHl r IHr|f [] v IHv] in e|-*.
+  - now right.
+  - apply Hdec.
+  - cbn. now apply impl_dec.
+  - cbn. apply fin_dec. 1:easy. intros k. apply IHv.
+  Qed.
+End decidable.
+
+
+#[global]
+Existing Instance falsity_on.
