theories/FOL/Semantics/FiniteTarski/Full.v
@@ -1,27 +1,14 @@
 From Undecidability.FOL.Semantics Require Import Tarski.FullFacts.
+From Undecidability.FOL.Semantics Require Export FiniteTarski.Listability.
 From Undecidability.FOL.Syntax Require Import Facts.
 Require Import Undecidability.Synthetic.DecidabilityFacts.
-Require Import Undecidability.Synthetic.EnumerabilityFacts.
+Require Import Undecidability.Shared.Dec.
 Require Import List.
-
-#[global]
-Existing Instance falsity_on.
-
-(* Definition of finiteness *)
-
-Definition listable X :=
-  exists L, forall x : X, In x L.
-
-Lemma listable_enumerable X :
-  listable X -> enumerable__T X.
-Proof.
-  intros [L HL]. exists (nth_error L).
-  intros x. apply In_nth_error, HL.
-Qed.
 
 Section DefaultSyntax. (* An alternative development of FSAT in Trakhtenbrot is "Trakhtenbrot Syntax" *)
   Context {Σ_funcs : funcs_signature}.
   Context {Σ_preds : preds_signature}.
+  Context {ff : falsity_flag}.
 
   (* Satisfiability in a finite and decidable model *)
 
@@ -46,3 +33,27 @@ Section DefaultSyntax. (* An alternative development of FSAT in Trakhtenbrot is 
   Definition FSATdc (phi : cform) :=
     FSATd (proj1_sig phi).
 End DefaultSyntax.
+
+Section decidable.
+  Context {Σ_funcs : funcs_signature}.
+  Context {Σ_preds : preds_signature}.
+  Context {ff : falsity_flag}.
+
+  (* Show satisfaction decidable for fixed model *)
+  Lemma general_decider D (I:interp D) (e : env D) f : cListable D -> (forall (ff:falsity_flag) p v ee, dec (ee ⊨ atom p v)) -> dec (e ⊨ f).
+  Proof.
+  intros Hfin Hdec.
+  induction f as [|f p v|f [] l IHl r IHr|f [] v IHv] in e|-*.
+  - now right.
+  - apply Hdec.
+  - cbn. now apply and_dec.
+  - cbn. now apply or_dec.
+  - cbn. now apply impl_dec.
+  - cbn. apply fin_dec. 1:easy. intros k. apply IHv.
+  - cbn. apply fin_dec_ex. 1:easy. intros k. apply IHv.
+  Qed.
+End decidable.
+
+
+#[global]
+Existing Instance falsity_on.
