theories/FOL/Semantics/FiniteTarski/DoubleNegation.v
@@ -184,6 +184,87 @@ Section translation.
       * intros [d Hd] Hc. contradict Hd. destruct (IHs (d.:rho)) as [IH1 [IH2 [IH3 IH4]]]. rewrite <- IH2. apply Hc.
     + intros term wterm ->. apply equiv_impl. firstorder.
   Qed.
+
+  Lemma translate_form_correct (f:falsity_flag) rho (phi : (@form _ _ full_operators f)) : 
+     (rho ⊨ translate_form phi <-> rho f⊨ phi).
+  Proof using Ddec.
+    apply correct.
+  Qed.
+
+  #[local] Hint Constructors bounded : core.
+(*
+  (* Show correctness by induction. *)
+  Lemma translate_bounded (f:falsity_flag)(phi : (@form _ _ full_operators f)) n : 
+     ((bounded n (translate_form phi) <-> bounded n phi)
+  /\ (bounded n (translate_negated phi) <-> bounded n phi))
+  /\ (forall wterm, bounded n (conj_to_impl_chain phi wterm) <-> (bounded n phi /\ bounded n wterm))
+  /\ (forall wterm, bounded n (disj_to_impl_chain phi wterm) <-> (bounded n phi /\ bounded n wterm)).
+  Proof.
+  induction phi as [|p v|f [| |] l IH r IH2|f [|] s IH] in n|-*; split; split; split; cbv; intros H; eauto.
+  - dependent inversion H. Search existT eq "dec".
+  - admit.
+  - 
+  - cbn. recsplit 3. 1-2:easy. 1-2:intros term wterm ->; tauto.
+  - recsplit 3.
+    + cbn. erewrite (Vector.map_ext). 1: apply eval_same_atom. apply eval_same.
+    + cbn. erewrite (Vector.map_ext). 1: apply equiv_impl; apply eval_same_atom. apply eval_same.
+    + intros term wterm H. cbn. rewrite <- eval_same_atom. rewrite <- H. erewrite (Vector.map_ext). 1:easy.  apply eval_same. 
+    + intros term wterm H. cbn. rewrite H. apply equiv_impl, equiv_impl. erewrite (Vector.map_ext). 1:apply eval_same_atom. apply eval_same.
+  - destruct (IHl rho) as [l1 [l2 [l3 l4]]], (IHr rho) as [r1 [r2 [r3 r4]]]. recsplit 3.
+    + cbn. rewrite l3. 2:easy. rewrite r3. 2:easy. split.
+      * intros H. destruct (Ddec l rho) as [Hl|Hnl], (Ddec r rho) as [Hr|Hnr]. 1:easy. all:exfalso; apply H; intros Hcl Hcr; cbn; easy.
+      * intros [Hl Hr] H. now apply H.
+    + cbn. rewrite l3. 2:easy. rewrite r3. 2:easy. tauto.
+    + intros term wterm H. cbn. rewrite l3. 2:easy. rewrite r3. 2:easy. rewrite H. tauto.
+    + intros term wterm H. cbn. rewrite l3. 2:easy. rewrite r3. 2:easy. rewrite H. apply equiv_impl. tauto.
+  - destruct (IHl rho) as [l1 [l2 [l3 l4]]], (IHr rho) as [r1 [r2 [r3 r4]]]. 
+    cbn. recsplit 3.
+    + rewrite l4. 2:easy. rewrite r4. 2:easy.  split.
+      * intros H. destruct (Ddec l rho) as [Hl|Hnl], (Ddec r rho) as [Hr|Hnr]. 1-3:tauto.
+        exfalso. now apply H.
+      * tauto.
+    + rewrite l4. 2:easy. rewrite r4. 2:easy. tauto.
+    + intros term wterm H. rewrite l4. 2:easy. rewrite r4. 2:easy. rewrite H. apply equiv_impl. split. 2:tauto.
+      intros Hc. destruct (Ddec l rho) as [Hl|Hnl], (Ddec r rho) as [Hr|Hnr]. 1-3:tauto. exfalso. now apply Hc.
+    + intros term wtertranslate_formm H. rewrite l4. 2:easy. rewrite r4. 2:easy. rewrite H. tauto.
+  - destruct (IHl rho) as [l1 [l2 [l3 l4]]], (IHr rho) as [r1 [r2 [r3 r4]]].
+    cbn. rewrite l3. 2:easy. rewrite r1. recsplit 3.
+    + tauto.
+    + tauto.
+    + intros term wterm H. rewrite l3. 2:easy. rewrite H. rewrite r1. tauto.
+    + intros term wterm H. rewrite l3. 2:easy. rewrite H. rewrite r1. tauto.
+  - cbn. recsplit 3.
+    + split.  
+      * intros H d. destruct (IHs (d.:rho)) as [IH1 [IH2 [IH3 IH4]]]. rewrite <- IH1. apply H.
+      * intros H d. destruct (IHs (d.:rho)) as [IH1 [IH2 [IH3 IH4]]]. rewrite IH1. apply H.
+    + split. 
+      * intros Hc H. apply Hc. intros d. destruct (IHs (d.:rho)) as [IH1 [IH2 [IH3 IH4]]]. rewrite IH1. apply H.
+      * intros Hc H. apply Hc. intros d. destruct (IHs (d.:rho)) as [IH1 [IH2 [IH3 IH4]]]. rewrite <- IH1. apply H.
+    + intros term wterm ->. split.
+      * intros Hc H. apply Hc. intros d. destruct (IHs (d.:rho)) as [IH1 [IH2 [IH3 IH4]]]. rewrite IH1. apply H.
+      * intros Hc H. apply Hc. intros d. destruct (IHs (d.:rho)) as [IH1 [IH2 [IH3 IH4]]]. rewrite <- IH1. apply H.
+    + intros term wterm ->. split.
+      * intros Hc H. apply Hc. intros Hcc. apply H. intros d. destruct (IHs (d.:rho)) as [IH1 [IH2 [IH3 IH4]]]. rewrite <- IH1. apply Hcc.
+      * intros Hc H. apply Hc. intros Hcc. apply H. intros d. destruct (IHs (d.:rho)) as [IH1 [IH2 [IH3 IH4]]]. rewrite IH1. apply Hcc.
+  - cbn. recsplit 3.
+    + split.
+      * intros H. destruct (Ddec (∃ s) rho) as [[e He]|Hne].
+        -- now exists e.
+        -- exfalso. apply H. intros d. destruct (IHs (d.:rho)) as [IH1 [IH2 [IH3 IH4]]].
+           rewrite IH2. intros Hc. apply Hne. now exists d.
+      * intros [d Hd] Hc. contradict Hd. destruct (IHs (d.:rho)) as [IH1 [IH2 [IH3 IH4]]]. rewrite <- IH2. apply Hc.
+    + split.
+      * intros Hc [d Hd]. contradict Hd.  destruct (IHs (d.:rho)) as [IH1 [IH2 [IH3 IH4]]]. rewrite <- IH2. apply Hc.
+      * intros Hc d. destruct (IHs (d.:rho)) as [IH1 [IH2 [IH3 IH4]]]. rewrite IH2. intros H. apply Hc. now exists d.
+    + intros term wterm ->. apply equiv_impl. split.
+      * intros H. destruct (Ddec (∃ s) rho) as [[e He]|Hne].
+        -- now exists e.
+        -- exfalso. apply H. intros d. destruct (IHs (d.:rho)) as [IH1 [IH2 [IH3 IH4]]].
+           rewrite IH2. intros Hc. apply Hne. now exists d.
+      * intros [d Hd] Hc. contradict Hd. destruct (IHs (d.:rho)) as [IH1 [IH2 [IH3 IH4]]]. rewrite <- IH2. apply Hc.
+    + intros term wterm ->. apply equiv_impl. firstorder.
+  Qed. *)
+
 End translation.
 
 
