theories/FOL/Undecidability/FSAT_undec.v
@@ -1,29 +1,97 @@
 From Undecidability.TRAKHTENBROT Require Import bpcp red_undec fo_sig.
 From Undecidability.Synthetic Require Import Undecidability ReducibilityFacts.
-From Undecidability.FOL.Semantics.FiniteTarski Require Import Full.
+From Undecidability.FOL.Syntax Require Import Core.
+From Undecidability.FOL.Semantics.FiniteTarski Require Fragment Full DoubleNegation.
 From Undecidability.FOL.Undecidability Require Import Reductions.FSATd_to_FSATdc Reductions.TRAKHTENBROT_to_FSAT.
 
-Theorem FSAT_undec :
-  undecidable FSAT.
-Proof.
-  apply (undecidability_from_reducibility BPCP_problem_undec).
-  eapply reduces_transitive; try apply reduction. 
-  apply (@FULL_TRAKHTENBROT_non_informative (Σrel 2)). left. exists tt. auto.
-Qed.
+Section Full.
+  Import Full.
 
-Theorem FSATd_undec :
-  undecidable FSATd.
-Proof.
-  apply (undecidability_from_reducibility BPCP_problem_undec).
-  eapply reduces_transitive; try apply reduction_disc.
-  eapply reduces_transitive; try apply (@FULL_TRAKHTENBROT_non_informative (Σrel 2)).
-  - left. exists tt. auto.
-  - exists (fun phi => phi). intros phi. apply red_utils.fo_form_fin_dec_SAT_discr_equiv.
-Qed.
+  Theorem FSAT_undec :
+    undecidable FSAT.
+  Proof.
+    apply (undecidability_from_reducibility BPCP_problem_undec).
+    eapply reduces_transitive; [| apply reduction].
+    apply (@FULL_TRAKHTENBROT_non_informative (Σrel 2)). left. exists tt. auto.
+  Qed.
 
-Theorem FSATdc_undec :
-  undecidable FSATdc.
-Proof.
- apply (undecidability_from_reducibility FSATd_undec).
- apply FSATd_to_FSATdc.reduction.
-Qed.
+  Theorem FSATd_undec :
+    undecidable FSATd.
+  Proof.
+    apply (undecidability_from_reducibility BPCP_problem_undec).
+    eapply reduces_transitive; try apply reduction_disc.
+    eapply reduces_transitive; try apply (@FULL_TRAKHTENBROT_non_informative (Σrel 2)).
+    - left. exists tt. auto.
+    - exists (fun phi => phi). intros phi. apply red_utils.fo_form_fin_dec_SAT_discr_equiv.
+  Qed.
+
+  Theorem FSATdc_undec :
+    undecidable FSATdc.
+  Proof.
+   apply (undecidability_from_reducibility FSATd_undec).
+   apply FSATd_to_FSATdc.reduction.
+  Qed.
+End Full.
+
+Section Fragment.
+  Import Fragment DoubleNegation.
+
+  Theorem FSAT_undec_frag :
+    undecidable FSAT.
+  Proof.
+    apply (undecidability_from_reducibility (FSAT_undec)).
+    exists translate_form.
+    intros k. split; intros (D & I & rho & (l & Hlist) & Hdec & H).
+    - exists D, (full_tarski_tarski_interp I), rho; repeat split.
+      + now exists l.
+      + destruct I; apply Hdec.
+      + rewrite <- (full_interp_inverse_1 I) in H.
+        destruct (Hdec tt) as [f Hf].
+        unshelve now eapply translate_form_correct in H.
+        intros ff phi rho'. apply Full.general_decider. 1: now exists l.
+        rewrite full_interp_inverse_1. intros ff' [] v ee. cbn.
+        apply DecidabilityFacts.decidable_iff'. now exists f.
+    - exists D, (tarski_full_tarski_interp I), rho; repeat split.
+      + now exists l.
+      + destruct I; apply Hdec.
+      + destruct (Hdec tt) as [f Hf].
+        unshelve now eapply translate_form_correct.
+        intros ff phi rho'. apply Full.general_decider. 1: now exists l.
+        intros ff' [] v ee. cbn.
+        apply DecidabilityFacts.decidable_iff'. destruct I. now exists f.
+  Qed.
+
+  Theorem FSATd_undec_frag :
+    undecidable FSATd.
+  Proof.
+    apply (undecidability_from_reducibility (FSATd_undec)).
+    exists translate_form.
+    intros k. split; intros (D & I & rho & (l & Hlist) & Hdisc & Hdec & H).
+    - exists D, (full_tarski_tarski_interp I), rho; repeat split.
+      + now exists l.
+      + easy.
+      + destruct I; apply Hdec.
+      + rewrite <- (full_interp_inverse_1 I) in H.
+        destruct (Hdec tt) as [f Hf].
+        unshelve now eapply translate_form_correct in H.
+        intros ff phi rho'. apply Full.general_decider. 1: now exists l.
+        rewrite full_interp_inverse_1. intros ff' [] v ee. cbn.
+        apply DecidabilityFacts.decidable_iff'. now exists f.
+    - exists D, (tarski_full_tarski_interp I), rho; repeat split.
+      + now exists l.
+      + easy.
+      + destruct I; apply Hdec.
+      + destruct (Hdec tt) as [f Hf].
+        unshelve now eapply translate_form_correct.
+        intros ff phi rho'. apply Full.general_decider. 1: now exists l.
+        intros ff' [] v ee. cbn.
+        apply DecidabilityFacts.decidable_iff'. destruct I. now exists f.
+  Qed.
+(* TODO 
+  Theorem FSATdc_undec :
+    undecidable FSATdc.
+  Proof.
+   apply (undecidability_from_reducibility FSATd_undec).
+   apply FSATd_to_FSATdc.reduction.
+  Qed. *)
+End Fragment.
