theories/FOL/Undecidability/minFOL_undec.v
@@ -2,7 +2,8 @@
 
 From Undecidability.DiophantineConstraints Require Import H10C H10C_undec.
 From Undecidability.FOL.Syntax Require Import Core BinSig.
-From Undecidability.FOL Require Semantics.Tarski.FragmentFacts Deduction.FragmentNDFacts Semantics.Kripke.FragmentCore Semantics.FiniteTarski.Fragment.
+From Undecidability.FOL Require Semantics.Tarski.FragmentFacts Deduction.FragmentNDFacts Semantics.Kripke.FragmentCore
+                                Semantics.FiniteTarski.Fragment.
 From Undecidability.FOL Require Semantics.Tarski.FragmentFacts Deduction.FullNDFacts.
 From Undecidability.FOL.Undecidability.Reductions Require H10UPC_to_FOL_minimal.
 From Undecidability.FOL.Undecidability.Reductions Require H10UPC_to_FOL_full_fragment H10UPC_to_FSAT.
@@ -74,19 +75,7 @@ Section finite.
   Import H10UPC_to_FSAT.
   Import Semantics.FiniteTarski.Fragment.
   Import Semantics.Tarski.FragmentFacts.
-  (* Reduction into fragment syntax. Step 1: define FSAT for fragment syntax *)
-  Definition FSAT_frag (phi : minimalForm falsity_on) :=
-  exists D (I : interp D) rho, listable D /\ decidable (fun v => i_atom (P:=tt) v) /\ @sat _ _ D I _ rho phi.
-
-  (* Also define FVAL for fragment syntax *)
-  Definition FVAL_frag (phi : minimalForm falsity_on) :=
-  forall D (I : interp D) rho, listable D /\ decidable (fun v => i_atom (P:=tt) v) -> @sat _ _ D I _ rho phi.
-
-  (* Also define FVAL for negation-free fragment *)
-  Definition FVAL_frag_no_negation (phi : minimalForm falsity_off) :=
-  forall D (I : interp D) rho, listable D /\ decidable (fun v => i_atom (P:=tt) v) -> @sat _ _ D I _ rho phi.
-
-  Lemma minFiniteSatisfiabilityUndec : undecidable FSAT_frag.
+  Lemma minFiniteSatisfiabilityUndec : undecidable FSAT.
   Proof.
     apply (undecidability_from_reducibility H10UPC_SAT_undec).
     eapply reduces_transitive.
@@ -94,7 +83,7 @@ Section finite.
     * eexists. apply frag_reduction_fsat.
   Qed.
 
-  Lemma minFiniteValidityUndec : undecidable FVAL_frag.
+  Lemma minFiniteValidityUndec : undecidable FVAL.
   Proof.
     apply (undecidability_from_reducibility H10UPC_SAT_compl_undec).
     eapply reduces_transitive.
@@ -103,7 +92,7 @@ Section finite.
   Qed.
 
   (* This is a conjecture *)
-  Lemma minFiniteValidityConjecture : undecidable FVAL_frag_no_negation.
+  Lemma minFiniteValidityConjecture : undecidable (@FVAL _ _ falsity_off).
   Abort.
 
 End finite.
